seplogic: prove parallel composition of traces is transitive

Semantics.thy
@@ -12,7 +12,12 @@ type_synonym 'a pred = \<open>'a \<Rightarrow> bool\<close>
 
 datatype (\<alpha>set: 'a) trace =
   TNil
-| TCons (trhd: 'a) (trtl: "'a trace") (infixr "\<cdot>" 70)
+  | TCons (trhd: 'a) (trtl: "'a trace") (infixr "\<cdot>" 70)
+  for
+    map: trace_map
+    pred: trace_all    
+    rel: trace_all2
+    
 
 lemma not_TNil_eq: \<open>a \<noteq> TNil \<longleftrightarrow> (\<exists>ax a'. a = ax \<cdot> a')\<close>
   using trace.exhaust_sel by blast
@@ -61,22 +66,20 @@ lemma merge_traces_rel_nil_simps[simp]:
   using merge_traces_rel_left_TNilD merge_traces_rel_right_TNilD
   by blast+
 
-lemma merge_traces_rel_cons_iff:
-  \<open>merge_traces_rel (x \<cdot> a') b c \<longleftrightarrow>
-    (\<exists>c'. merge_traces_rel a' b c' \<and> c = x \<cdot> c') \<or>
-      (\<exists>y b' c'. merge_traces_rel (x \<cdot> a') b' c' \<and> b = y \<cdot> b' \<and> c = y \<cdot> c')\<close>
-  \<open>merge_traces_rel a (y \<cdot> b') c \<longleftrightarrow>
-    (\<exists>c'. merge_traces_rel a b' c' \<and> c = y \<cdot> c') \<or>
-      (\<exists>x a' c'. merge_traces_rel a' (y \<cdot> b') c' \<and> a = x \<cdot> a' \<and> c = x \<cdot> c')\<close>
-   apply (metis mergetr_cons_left mergetr_cons_right mergetr_left_consE)
-  apply (metis mergetr_cons_left mergetr_cons_right mergetr_right_consE)
+lemma merge_traces_rel_cons_LR_iff:
+  \<open>merge_traces_rel (x \<cdot> a') (y \<cdot> b') c \<longleftrightarrow>
+    (\<exists>c'. merge_traces_rel a' (y \<cdot> b') c' \<and> c = x \<cdot> c') \<or>
+    (\<exists>c'. merge_traces_rel (x \<cdot> a') b' c' \<and> c = y \<cdot> c')\<close>
+  apply (induct c)
+   apply force
+  apply (simp, metis mergetr_cons_left mergetr_cons_right mergetr_out_consE trace.inject)
   done
 
-lemma merge_traces_rel_cons_simps[simp]:
+lemma merge_traces_rel_cons_out_iff:
   \<open>merge_traces_rel a b (z \<cdot> c') \<longleftrightarrow>
     (\<exists>a'. merge_traces_rel a' b c' \<and> a = z \<cdot> a') \<or>
     (\<exists>b'. merge_traces_rel a b' c' \<and> b = z \<cdot> b')\<close>
-  by (meson mergetr_cons_left mergetr_cons_right mergetr_out_consE)
+  by (metis mergetr_cons_left mergetr_cons_right mergetr_out_consE)
 
 lemma merge_traces_assoc1:
   assumes
@@ -87,16 +90,13 @@ lemma merge_traces_assoc1:
     \<open>\<exists>a b c bc. a \<in> A \<and> b \<in> B \<and> c \<in> C \<and> merge_traces_rel b c bc \<and> merge_traces_rel a bc abc\<close>
   using assms
 proof (induct abc arbitrary: a b ab c A B C)
-  case TNil
-  then show ?case
-    by simp
-next
   case (TCons x abc)
   then show ?case
-    apply clarsimp
+    apply (clarsimp simp add: merge_traces_rel_cons_out_iff)
     apply (erule disjE)
-     apply clarsimp
+     apply (clarsimp simp add: merge_traces_rel_cons_out_iff)
      apply (erule disjE)
+      (* Case: \<open>a\<close> takes a step *)
       apply clarsimp
       apply (rename_tac ab' a')
       apply (drule meta_spec, drule meta_spec, drule meta_spec, drule meta_spec)
@@ -104,22 +104,28 @@ next
       apply (drule_tac x=B in meta_spec)
       apply (drule_tac x=C in meta_spec)
       apply blast
+      (* Case: \<open>b\<close> takes a step *)
      apply clarsimp
      apply (rename_tac ab' b')
-     apply (drule meta_spec, drule meta_spec, drule meta_spec, drule meta_spec)
-     apply (drule_tac x=A in meta_spec)
-     apply (drule_tac x=\<open>{a. x \<cdot> a \<in> B}\<close> in meta_spec)
-     apply (drule_tac x=C in meta_spec)
-     apply force
+     apply (drule meta_spec[of _ a], drule meta_spec, drule meta_spec, drule meta_spec)
+     apply (drule meta_spec[of _ A])
+     apply (drule meta_spec[of _ \<open>{a. x \<cdot> a \<in> B}\<close>])
+     apply (drule meta_spec[of _ C])
+     apply (drule meta_mp, assumption)
+     apply (drule meta_mp, assumption)
+     apply (metis mem_Collect_eq mergetr_cons_left)
+      (* Case: \<open>c\<close> takes a step *)
     apply clarsimp
     apply (rename_tac c')
-    apply (drule meta_spec, drule meta_spec, drule meta_spec, drule meta_spec)
+    apply (drule meta_spec[of _ a], drule meta_spec, drule meta_spec, drule meta_spec)
     apply (drule_tac x=A in meta_spec)
     apply (drule_tac x=B in meta_spec)
     apply (drule_tac x=\<open>{c. x \<cdot> c \<in> C}\<close> in meta_spec)
-    apply force
+    apply (drule meta_mp, assumption)
+    apply (drule meta_mp, assumption)
+    apply (metis mem_Collect_eq mergetr_cons_right)
     done
-qed
+qed simp
 
 
 lemma merge_traces_assoc2:
@@ -128,69 +134,114 @@ lemma merge_traces_assoc2:
     \<open>merge_traces_rel a bc abc\<close>
     \<open>a \<in> A\<close> \<open>b \<in> B\<close> \<open>c \<in> C\<close>
   shows
-    \<open>\<exists>a b c bc. a \<in> A \<and> b \<in> B \<and> c \<in> C \<and> merge_traces_rel b c bc \<and> merge_traces_rel a bc abc\<close>
+    \<open>\<exists>a b c ab. a \<in> A \<and> b \<in> B \<and> c \<in> C \<and> merge_traces_rel a b ab \<and> merge_traces_rel ab c abc\<close>
   using assms
 proof (induct abc arbitrary: a b c bc A B C)
-  case TNil
-  then show ?case
-    by simp
-next
   case (TCons x abc)
   then show ?case
-    apply clarsimp
+    apply (clarsimp simp add: merge_traces_rel_cons_out_iff)
     apply (erule disjE)
      apply clarsimp
-     apply (erule disjE)
-      apply clarsimp
-      apply (rename_tac ab' a')
-      apply (drule meta_spec, drule meta_spec, drule meta_spec, drule meta_spec)
-      apply (drule_tac x=\<open>{a. x \<cdot> a \<in> A}\<close> in meta_spec)
-      apply (drule_tac x=B in meta_spec)
-      apply (drule_tac x=C in meta_spec)
-      apply blast
+      (* Case: \<open>a\<close> takes a step *)
+     apply (drule meta_spec[of _ b], drule meta_spec, drule meta_spec, drule meta_spec)
+     apply (drule meta_spec[of _ \<open>{t. x \<cdot> t \<in> A}\<close>])
+     apply (drule meta_spec[of _ B])
+     apply (drule meta_spec[of _ C])
+     apply (drule meta_mp, assumption)
+     apply (drule meta_mp, assumption)
+     apply (simp, metis mergetr_cons_left)
+    apply (clarsimp simp add: merge_traces_rel_cons_out_iff)
+    apply (erule disjE)
+      (* Case: \<open>b\<close> takes a step *)
      apply clarsimp
      apply (rename_tac ab' b')
-     apply (drule meta_spec, drule meta_spec, drule meta_spec, drule meta_spec)
-     apply (drule_tac x=A in meta_spec)
-     apply (drule_tac x=\<open>{a. x \<cdot> a \<in> B}\<close> in meta_spec)
-     apply (drule_tac x=C in meta_spec)
-     apply force
+     apply (drule meta_spec, drule meta_spec[of _ c], drule meta_spec, drule meta_spec)
+     apply (drule meta_spec[of _ A])
+     apply (drule meta_spec[of _ \<open>{t. x \<cdot> t \<in> B}\<close>])
+     apply (drule meta_spec[of _ C])
+     apply (drule meta_mp, assumption)
+     apply (drule meta_mp, assumption)
+     apply (simp, metis mergetr_cons_right)
+      (* Case: \<open>c\<close> takes a step *)
     apply clarsimp
     apply (rename_tac c')
-    apply (drule meta_spec, drule meta_spec, drule meta_spec, drule meta_spec)
-    apply (drule_tac x=A in meta_spec)
-    apply (drule_tac x=B in meta_spec)
-    apply (drule_tac x=\<open>{c. x \<cdot> c \<in> C}\<close> in meta_spec)
-    apply force
+    apply (drule meta_spec[of _ b], drule meta_spec, drule meta_spec, drule meta_spec)
+    apply (drule meta_spec[of _ A])
+    apply (drule meta_spec[of _ B])
+    apply (drule meta_spec[of _ \<open>{t. x \<cdot> t \<in> C}\<close>])
+    apply blast
     done
+qed simp
+
+lemma merge_traces_rel_assoc:
+  \<open>{abc. \<exists>a. a \<in> A \<and> (\<exists>b. b \<in> B \<and> (\<exists>c. c \<in> C \<and> (\<exists>ab.
+      merge_traces_rel a b ab \<and> merge_traces_rel ab c abc)))}
+    = {abc. \<exists>a. a \<in> A \<and> (\<exists>b. b \<in> B \<and> (\<exists>c. c \<in> C \<and> (\<exists>bc.
+        merge_traces_rel b c bc \<and> merge_traces_rel a bc abc)))}\<close>
+  using merge_traces_assoc1 merge_traces_assoc2
+  by fast
+
+definition merge_traces :: \<open>'a trace \<Rightarrow> 'a trace \<Rightarrow> 'a trace set\<close> where
+  \<open>merge_traces a b \<equiv> Collect (merge_traces_rel a b)\<close>
+
+fun tmp :: \<open>'a trace \<Rightarrow> 'a trace \<Rightarrow> 'a trace set\<close> where
+  \<open>tmp TNil b = {b}\<close>
+| \<open>tmp a TNil = {a}\<close>
+| \<open>tmp (x \<cdot> a) (y \<cdot> b) = ((TCons x ` tmp a (y \<cdot> b)) \<union> (TCons y ` tmp (x \<cdot> a) b))\<close>
+
+lemma merge_traces_simp[simp]:
+  \<open>merge_traces TNil b = {b}\<close>
+  \<open>merge_traces a TNil = {a}\<close>
+  \<open>merge_traces (x \<cdot> a) (y \<cdot> b) =
+    ((TCons x ` merge_traces a (y \<cdot> b)) \<union> (TCons y ` merge_traces (x \<cdot> a) b))\<close>
+    apply (force simp add: merge_traces_def)
+   apply (force simp add: merge_traces_def)
+  apply (force simp add: merge_traces_def set_eq_iff merge_traces_rel_cons_LR_iff image_def)
+  done
+
+lemma traces2_step_induct[case_names TNil2 TConsL TConsR]:
+  \<open>P TNil TNil \<Longrightarrow>
+    (\<And>a b x. P a b \<Longrightarrow> P (x \<cdot> a) b) \<Longrightarrow>
+    (\<And>a b y. P a b \<Longrightarrow> P a (y \<cdot> b)) \<Longrightarrow>
+    P a b\<close>
+proof (induct a arbitrary: b)
+  case (TNil b)
+  then show ?case
+    by (induct b) blast+
+next
+  case TCons
+  then show ?case
+    by blast
 qed
 
-lemma merge_traces_assoc:
-  \<open>{abc|a b c ab abc::'a trace. a \<in> A \<and> b \<in> B \<and> c \<in> C \<and> merge_traces_rel a b ab \<and> merge_traces_rel ab c abc} =
-    {abc|a b c bc abc. a \<in> A \<and> b \<in> B \<and> c \<in> C \<and> merge_traces_rel b c bc \<and> merge_traces_rel a bc abc}\<close>
-  sorry
-
-(*
-fun merge_traces :: \<open>'a trace \<Rightarrow> 'a trace \<Rightarrow> 'a trace set\<close> where
-  \<open>merge_traces TNil b = {b}\<close>
-| \<open>merge_traces a TNil = {a}\<close>
-| \<open>merge_traces (x \<cdot> a) (y \<cdot> b) = (\<Union>t\<in>merge_traces a b. {x \<cdot> y \<cdot> t, y \<cdot> x \<cdot> t})\<close>
-
-lemmas merge_traces_induct = merge_traces.induct[case_names LeftTNil RightTNil TCons]
-
-lemma merge_traces_extra_simps[simp]:
-  \<open>merge_traces a TNil = {a}\<close>
-  by (metis merge_traces.simps(1,2) not_TNil_eq)
+lemma merge_traces_induct[case_names TNilL TNilR TCons2]:
+  \<open>(\<And>b. P TNil b) \<Longrightarrow>
+    (\<And>a. P a TNil) \<Longrightarrow>
+    (\<And>a b x y.
+      P a (y \<cdot> b) \<Longrightarrow>
+      P (x \<cdot> a) b \<Longrightarrow>
+      P (x \<cdot> a) (y \<cdot> b)) \<Longrightarrow>
+    P a b\<close>
+proof (induct a arbitrary: b)
+  case TNil
+  then show ?case
+    by blast
+next
+  case (TCons x a b)
+  then show ?case
+    by (induct b) blast+
+qed
 
 lemma TNil_merge_traces_TNil_parts:
   \<open>TNil \<in> merge_traces a b \<Longrightarrow> a = TNil \<or> b = TNil\<close>
-  by (induct a b rule: merge_traces.induct) force+
+  by (simp add: merge_traces_def)
 
 lemma merge_traces_assoc:
-  \<open>{abc|a b c ab abc::'a trace. a \<in> A \<and> b \<in> B \<and> c \<in> C \<and> ab \<in> merge_traces a b \<and> abc \<in> merge_traces ab c} =
-    {abc|a b c bc abc. a \<in> A \<and> b \<in> B \<and> c \<in> C \<and> bc \<in> merge_traces b c \<and> abc \<in> merge_traces a bc}\<close>
-  sorry
-*)
+  \<open>{abc|a b c ab abc::'a trace.
+      a \<in> A \<and> b \<in> B \<and> c \<in> C \<and> ab \<in> merge_traces a b \<and> abc \<in> merge_traces ab c}
+    = {abc|a b c bc abc.
+        a \<in> A \<and> b \<in> B \<and> c \<in> C \<and> bc \<in> merge_traces b c \<and> abc \<in> merge_traces a bc}\<close>
+  by (simp add: merge_traces_def merge_traces_rel_assoc)
 
 section \<open>Processes\<close>
 
@@ -202,7 +253,7 @@ instantiation process :: (type) monoid_mult
 begin
 
 definition times_process :: \<open>'a process \<Rightarrow> 'a process \<Rightarrow> 'a process\<close> where
-  \<open>times_process A B \<equiv> Process (\<Union>{merge_traces a b|a b. a \<in> proctr A \<and> b \<in> proctr B })\<close>
+  \<open>times_process A B \<equiv> Process (\<Union>(a,b) \<in> (proctr A \<times> proctr B). merge_traces a b)\<close>
 
 definition one_process :: \<open>'a process\<close> where
   \<open>one_process \<equiv> Process {TNil}\<close>
@@ -212,7 +263,7 @@ proof
   fix a b c :: \<open>'a process\<close>
   show \<open>a \<parallel> b \<parallel> c = a \<parallel> (b \<parallel> c)\<close>
     apply (simp add: times_process_def one_process_def Setcompr_eq_image Union_eq)
-    apply (rule HOL.trans[OF _ merge_traces_assoc[where A=\<open>proctr a\<close> and B=\<open>proctr b\<close> and C=\<open>proctr c\<close>], THEN HOL.trans])
+    apply (rule HOL.trans[OF _ merge_traces_assoc, THEN HOL.trans])
      apply blast
     apply blast
     done
